WIP convert CQueue: define vprops

examples/steel/CQueue.Cell.fst
@@ -23,16 +23,87 @@ let ccell_data #a c =
 let ccell_next #a c =
   c.next
 
+let vptr_pts_to
+  (#opened: _)
+  (#a: Type)
+  (r: ref a)
+: SteelGhost (Ghost.erased a) opened
+    (vptr r)
+    (fun v -> pts_to r full_perm v)
+    (fun _ -> True)
+    (fun h v _ -> Ghost.reveal v == h (vptr r))
+=
+  let v = gget (vptr r) in
+  change_slprop
+    (vptr r)
+    (pts_to r full_perm v)
+    v
+    (Ghost.hide ())
+    (fun m -> ptr_sel_interp r m);
+  v
+
 #push-options "--ide_id_info_off"
+
+// FIXME: WHY WHY WHY are the following two SO slow, even with the assumes? (and WHY WHY WHY do they fail without them?)
+
+let ccell_full_ccell
+  #opened #a c
+=
+  let res : Ghost.erased (vcell a) = gget (ccell_full c) in
+  elim_vrewrite
+    (vptr (ccell_data c) `star` vptr (ccell_next c))
+    (ccell_rewrite c);
+  reveal_star (vptr (ccell_data c)) (vptr (ccell_next c));
+  let vdata : Ghost.erased a = vptr_pts_to (ccell_data c) in
+  assert (Ghost.reveal vdata == (Ghost.reveal res).vcell_data);
+  assert (vdata == Ghost.hide (Ghost.reveal res).vcell_data);
+  let vnext : Ghost.erased (ccell_ptrvalue a) = vptr_pts_to (ccell_next c) in
+  assert (Ghost.reveal vnext == (Ghost.reveal res).vcell_next);
+  assert (vnext == Ghost.hide (Ghost.reveal res).vcell_next);
+(* // wtf congruence?
+  assert (
+    pts_to (ccell_data c) full_perm vdata ==
+    pts_to (ccell_data c) full_perm (Ghost.hide  (Ghost.reveal res).vcell_data)
+  );
+  assert (
+    pts_to (ccell_next c) full_perm vnext ==
+    pts_to (ccell_next c) full_perm (Ghost.hide (Ghost.reveal res).vcell_next)
+  );
+*)
+  assume (
+    (pts_to (ccell_data c) full_perm vdata `star` pts_to (ccell_next c) full_perm vnext) ==
+    (ccell c full_perm res)
+  );
+  change_equal_slprop
+    (pts_to (ccell_data c) full_perm vdata `star` pts_to (ccell_next c) full_perm vnext)
+    (ccell c full_perm res);
+  res
+
+let alloc_cell_full
+  #a data next
+=
+  let rdata = alloc data in
+  let vdata = gget (vptr rdata) in
+  assume (Ghost.reveal vdata == data);
+  let rnext = alloc next in
+  let vnext = gget (vptr rnext) in
+  assume (Ghost.reveal vnext == next);
+  let res : ccell_lvalue a = ({ data = rdata; next = rnext; all_or_none_null = () }) in
+  change_equal_slprop (vptr rdata) (vptr (ccell_data res));
+  change_equal_slprop (vptr rnext) (vptr (ccell_next res));
+  reveal_star (vptr (ccell_data res)) (vptr (ccell_next res));
+  intro_vrewrite (vptr (ccell_data res) `star` vptr (ccell_next res)) (ccell_rewrite res);
+  return res
 
 let alloc_cell
   #a data next
 =
-  let rdata = alloc_pt data in
-  let rnext = alloc_pt next in
-  let gres = Ghost.hide ({ vcell_data = data; vcell_next = next }) in
-  let res = ({ data = rdata; next = rnext; all_or_none_null = () }, gres) in
-  rewrite_slprop (pts_to rdata full_perm data `star` pts_to rnext full_perm next) (ccell (fst res) full_perm (snd res)) (fun _ -> ());
+  let pc = alloc_cell_full data next in
+  let vc = ccell_full_ccell pc in
+  let res = (pc, vc) in
+  change_equal_slprop
+    (ccell pc full_perm vc)
+    (ccell (fst res) full_perm (snd res));
   return res
 
 let free_cell
